propagate step 2.1

src/Std/Tactic/BVDecide/Bitblast/BVExpr/Circuit/Impl.lean
@@ -4,8 +4,7 @@ Released under Apache 2.0 license as described in the file LICENSE.
 Authors: Henrik Böving
 -/
 prelude
-import Std.Tactic.BVDecide.Bitblast.BVExpr.Circuit.Impl.Pred
-import Std.Tactic.BVDecide.Bitblast.BoolExpr.Circuit
+import Std.Tactic.BVDecide.Bitblast.BVExpr.Circuit.Impl.Substructure
 
 /-!
 This module contains the implementation of a bitblaster for general `BitVec` problems with boolean
@@ -19,7 +18,7 @@ open Std.Sat
 namespace BVLogicalExpr
 
 def bitblast (expr : BVLogicalExpr) : AIG.Entrypoint BVBit :=
-  ofBoolExprCached expr BVPred.bitblast
+  ofBoolExprCached expr
 
 end BVLogicalExpr
 
