src/Std/Tactic/BVDecide/Bitblast/BVExpr/Circuit/Impl/Pred.lean
@@ -18,80 +18,89 @@ namespace Std.Tactic.BVDecide
 
 open Std.Sat
 
+structure Return (aig : AIG BVBit) where
+  result : AIG.ExtendingEntrypoint aig
+  cache : BVExpr.Cache result.val.aig
+
 namespace BVPred
 
-def bitblast (aig : AIG BVBit) (pred : BVPred) : AIG.Entrypoint BVBit :=
-  let cache := BVExpr.Cache.empty
+def bitblast (aig : AIG BVBit) (input : BVExpr.WithCache BVPred aig) : Return aig :=
+  let ⟨pred, cache⟩ := input
   match pred with
   | .bin lhs op rhs =>
-    let ⟨⟨⟨aig, lhsRefs⟩, _⟩, cache⟩ := BVExpr.bitblast aig ⟨lhs, cache⟩
-    let ⟨⟨⟨aig, rhsRefs⟩, hrhs⟩, _⟩ := BVExpr.bitblast aig ⟨rhs, cache⟩
+    let ⟨⟨⟨aig, lhsRefs⟩, hlhs⟩, cache⟩ := BVExpr.bitblast aig ⟨lhs, cache⟩
+    let ⟨⟨⟨aig, rhsRefs⟩, hrhs⟩, cache⟩ := BVExpr.bitblast aig ⟨rhs, cache⟩
     let lhsRefs := lhsRefs.cast hrhs
     match op with
-    | .eq => mkEq aig ⟨lhsRefs, rhsRefs⟩
-    | .ult => mkUlt aig ⟨lhsRefs, rhsRefs⟩
+    | .eq =>
+      let res := mkEq aig ⟨lhsRefs, rhsRefs⟩
+      let cache := cache.cast (AIG.LawfulOperator.le_size (f := mkEq) ..)
+      have := by
+        apply AIG.LawfulOperator.le_size_of_le_aig_size (f := mkEq)
+        dsimp only at hlhs hrhs
+        omega
+      ⟨⟨res, this⟩, cache⟩
+    | .ult =>
+      let res := mkUlt aig ⟨lhsRefs, rhsRefs⟩
+      have := AIG.LawfulOperator.le_size (f := mkUlt) ..
+      let cache := cache.cast this
+      have := by
+        apply AIG.LawfulOperator.le_size_of_le_aig_size (f := mkUlt)
+        dsimp only at hlhs hrhs
+        omega
+      ⟨⟨res, this⟩, cache⟩
   | .getLsbD expr idx =>
     /-
     Note: This blasts the entire expression up to `w` despite only needing it up to `idx`.
     However the vast majority of operations are interested in all bits so the API is currently
     not designed to support this use case.
     -/
-    let ⟨⟨⟨aig, refs⟩, _⟩, _⟩ := BVExpr.bitblast aig ⟨expr, cache⟩
-    blastGetLsbD aig ⟨refs, idx⟩
-
-instance : AIG.LawfulOperator BVBit (fun _ => BVPred) bitblast where
-  le_size := by
-    intro aig pred
-    unfold BVPred.bitblast
-    cases pred with
-    | bin lhs op rhs =>
-      cases op with
-      | eq =>
-        dsimp only
-        apply AIG.LawfulOperator.le_size_of_le_aig_size (f := mkEq)
-        refine Nat.le_trans ?_ (BVExpr.bitblast_le_size ..)
-        apply BVExpr.bitblast_le_size
-      | ult =>
-        dsimp only
-        apply AIG.LawfulOperator.le_size_of_le_aig_size (f := mkUlt)
-        refine Nat.le_trans ?_ (BVExpr.bitblast_le_size ..)
-        apply BVExpr.bitblast_le_size
-    | getLsbD expr idx =>
-      dsimp only
+    let ⟨⟨⟨aig, refs⟩, hrefs⟩, cache⟩ := BVExpr.bitblast aig ⟨expr, cache⟩
+    let res := blastGetLsbD aig ⟨refs, idx⟩
+    let cache := cache.cast (AIG.LawfulOperator.le_size (f := blastGetLsbD) ..)
+    have := by
       apply AIG.LawfulOperator.le_size_of_le_aig_size (f := blastGetLsbD)
-      apply BVExpr.bitblast_le_size
-  decl_eq := by
-    intro aig pred idx h1 h2
-    unfold BVPred.bitblast
-    cases pred with
-    | bin lhs op rhs =>
-      cases op with
-      | eq =>
-        dsimp only
-        rw [AIG.LawfulOperator.decl_eq (f := mkEq)]
-        rw [BVExpr.bitblast_decl_eq]
-        rw [BVExpr.bitblast_decl_eq]
-        · apply BVExpr.bitblast_lt_size_of_lt_aig_size
-          assumption
-        · apply BVExpr.bitblast_lt_size_of_lt_aig_size
-          apply BVExpr.bitblast_lt_size_of_lt_aig_size
-          assumption
-      | ult =>
-        simp only [bitblast]
-        rw [AIG.LawfulOperator.decl_eq (f := mkUlt)]
-        rw [BVExpr.bitblast_decl_eq]
-        rw [BVExpr.bitblast_decl_eq]
-        · apply BVExpr.bitblast_lt_size_of_lt_aig_size
-          assumption
-        · apply BVExpr.bitblast_lt_size_of_lt_aig_size
-          apply BVExpr.bitblast_lt_size_of_lt_aig_size
-          assumption
-    | getLsbD expr idx =>
-      simp only [bitblast]
-      rw [AIG.LawfulOperator.decl_eq (f := blastGetLsbD)]
+      exact hrefs
+    ⟨⟨res, this⟩, cache⟩
+
+theorem bitblast_decl_eq (aig : AIG BVBit) (input : BVExpr.WithCache BVPred aig) :
+    ∀ (idx : Nat) (h1) (h2), (bitblast aig input).result.val.aig.decls[idx]'h2 = aig.decls[idx]'h1 := by
+  intro idx h1 h2
+  rcases input with ⟨pred, cache⟩
+  unfold BVPred.bitblast
+  cases pred with
+  | bin lhs op rhs =>
+    cases op with
+    | eq =>
+      dsimp only
+      rw [AIG.LawfulOperator.decl_eq (f := mkEq)]
       rw [BVExpr.bitblast_decl_eq]
-      apply BVExpr.bitblast_lt_size_of_lt_aig_size
-      assumption
+      rw [BVExpr.bitblast_decl_eq]
+      · apply BVExpr.bitblast_lt_size_of_lt_aig_size
+        assumption
+      · apply BVExpr.bitblast_lt_size_of_lt_aig_size
+        apply BVExpr.bitblast_lt_size_of_lt_aig_size
+        assumption
+    | ult =>
+      simp only [bitblast]
+      rw [AIG.LawfulOperator.decl_eq (f := mkUlt)]
+      rw [BVExpr.bitblast_decl_eq]
+      rw [BVExpr.bitblast_decl_eq]
+      · apply BVExpr.bitblast_lt_size_of_lt_aig_size
+        assumption
+      · apply BVExpr.bitblast_lt_size_of_lt_aig_size
+        apply BVExpr.bitblast_lt_size_of_lt_aig_size
+        assumption
+  | getLsbD expr idx =>
+    simp only [bitblast]
+    rw [AIG.LawfulOperator.decl_eq (f := blastGetLsbD)]
+    rw [BVExpr.bitblast_decl_eq]
+    apply BVExpr.bitblast_lt_size_of_lt_aig_size
+    assumption
+
+theorem bitblast_le_size (aig : AIG BVBit) (input : BVExpr.WithCache BVPred aig) :
+    aig.decls.size ≤ (bitblast aig input).result.val.aig.decls.size := by
+  exact (bitblast aig input).result.property
 
 end BVPred
 
